some hacking around MILP

examples/vipr/milpScript.sml
@@ -7,31 +7,24 @@ val _ = new_theory "milp";
 
 val _ = numLib.prefer_num();
 
-(* The left-hand side of a mixed linear constraint *)
-Type lin_term = ``:(rat # 'a) list # (rat # 'b) list ``;
+(* x |-> r *)
+Type lin_term = ``: real num_map``;
+(* x |-> r or i *)
+Type mix_val = ``: (num -> real) # (num -> int)``;
 
-(* A valuation maps 'a to reals and 'b to integers *)
-Type mix_val = ``: ('a -> real) # ('b -> int)``;
+Definition eval_real_term_def:
+  eval_real_term w (x,r:real) = (r * w x):real
+End
 
 Definition rSUM_def:
   (rSUM [] = 0:real) ∧
   (rSUM (x::xs) = x + rSUM xs)
 End
 
-Definition eval_rat_term_def:
-  eval_rat_term w (r:rat,x) = (real_of_rat r * w x):real
-End
-
-Definition eval_int_term_def:
-  eval_int_term w (r:rat,x) = (real_of_rat r * real_of_int (w x)):real
-End
-
 Definition eval_lhs_def:
-  eval_lhs
-    ((w1,w2): ('a,'b) mix_val)
-    ((xs,ys):('a,'b) lin_term) =
-    rSUM (MAP (eval_rat_term w1) xs) +
-    rSUM (MAP (eval_int_term w2) ys)
+  eval_lhs w lhs =
+    let xs = toAList lhs in
+    rSUM (MAP (eval_real_term w) xs)
 End
 
 (*
@@ -40,12 +33,12 @@ End
   c_i l_i = n
   c_i l_i ≤ n
 *)
-
 Datatype:
   linop = Equal | GreaterEqual | LessEqual
 End
 
-Type milc = ``:(linop # ('a,'b) lin_term # rat)``
+(* A linear constraint *)
+Type milc = ``:(linop # lin_term # real)``
 
 Definition do_op_def[simp]:
   (do_op Equal (l:real) (r:real) ⇔ l = r) ∧
@@ -55,93 +48,203 @@ End
 
 (* satisfaction of a mixed integer linear constraint *)
 Definition satisfies_milc_def:
-  (satisfies_milc w (lop,xs,n) ⇔
-    do_op lop (eval_lhs w xs) (real_of_rat n))
+  (satisfies_milc w (lop,lhs,n) ⇔
+    do_op lop (eval_lhs w lhs) n)
 End
 
 (* satisfaction of an MILP *)
 Definition satisfies_def:
-  satisfies w milp ⇔
-  ∀c. c ∈ milp ⇒ satisfies_milc w c
+  satisfies w intv milp ⇔
+  (∀v. v ∈ intv ⇒ is_int (w v)) ∧
+  (∀c. c ∈ milp ⇒ satisfies_milc w c)
 End
 
-(* Define floor and ceiling for rationals *)
-Definition RAT_INT_FLOOR_def[nocompute]:
-  RAT_INT_FLOOR r = INT_FLOOR (real_of_rat r)
+Datatype:
+  result = Infeasible | Range (real option) (real option)
 End
 
-Definition RAT_INT_CEILING_def[nocompute]:
-  RAT_INT_CEILING r = INT_CEILING (real_of_rat r)
-
+(* The assignment w gives an optimal value for min/max problem *)
+Definition optimal_def:
+  (optimal intv milp min obj w ⇔
+  satisfies w intv milp ∧
+  ∀w'.
+    satisfies w' intv milp ⇒
+    (min ⇒ eval_lhs w obj ≤ eval_lhs w' obj) ∧
+    (¬min ⇒ eval_lhs w' obj ≤ eval_lhs w obj)
+  )
 End
 
-Definition RAT_is_int_def:
-  RAT_is_int (x:rat) ⇔
-  x = rat_of_int (RAT_INT_FLOOR x)
+(*
+  intv: set of integer variables
+  milp: the MILP constraints
+  min: boolean flag, true to minimize obj (or maximize if false)
+  obj: objective linear term
+*)
+Definition rtp_def:
+  (rtp intv milp min obj Infeasible ⇔
+    ∀w. ¬satisfies w intv milp) ∧
+  (rtp intv milp min obj (Range lb ub) ⇔
+    (* Satisfiable *)
+    (∃w. satisfies w intv milp) ∧
+    ∀w. optimal intv milp min obj w ⇒
+      (case lb of NONE => T | SOME lb => lb ≤ eval_lhs w obj) ∧
+      (case ub of NONE => T | SOME ub => eval_lhs w obj ≤ ub))
 End
 
-(* Computing the int floor of a rational number *)
-Theorem RAT_INT_FLOOR_compute:
-  RAT_INT_FLOOR r =
-  RATN r / & RATD r
-Proof
-  rw[RAT_INT_FLOOR_def]>>
-  simp[RatProgTheory.real_of_rat_def]>>
-  Cases_on`RATN r`>>
-  simp[]>>
-  DEP_REWRITE_TAC[intrealTheory.INT_FLOOR_EQNS]>>
-  simp[]
-QED
+(* Implication constraints *)
+Definition satisfies_imp_milc_def:
+  satisfies_imp_milc w assms milc ⇔
+  ((∀c. c ∈ assms ⇒ satisfies_milc w c) ⇒ satisfies_milc w milc)
+End
 
-Theorem real_of_int_of_rat:
-  real_of_int i = real_of_rat (rat_of_int i)
-Proof
-  simp[real_of_rat_def]
-QED
+Definition satisfies_imp_milp_def:
+  satisfies_imp_milp w imilp ⇔
+  ∀i c. (i,c) ∈ imilp ⇒ satisfies_imp_milc w i c
+End
 
-Theorem RAT_INT_CEILING_compute:
-  RAT_INT_CEILING r =
-  let i = RAT_INT_FLOOR r in
-    if rat_of_int i = r then i else i + 1
-Proof
-  rw[RAT_INT_CEILING_def,RAT_INT_FLOOR_def]>>
-  fs[intrealTheory.INT_CEILING_INT_FLOOR]>>
-  fs[real_of_int_of_rat]
-QED
+(* Syntactic stuff *)
 
-(* Rounding up a constraint *)
-Definition round_up_def:
-  round_up ((xs,ys),n) =
-  if xs = [] then
-    if EVERY (λ(r,y). RAT_is_int r) ys then
-      SOME (rat_of_int (RAT_INT_CEILING n))
-    else NONE
+(* check a partial solution *)
+Definition check_dom_def:
+  check_dom (intv:num_set) (sol:real num_map) ⇔
+  let ls = toAList sol in
+  EVERY (λ(k,v). lookup k intv = SOME () ⇒ is_int v) ls
+End
+
+Definition mk_sol_def:
+  mk_sol sol x =
+  case lookup x sol of NONE => 0 | SOME r => (r:real)
+End
+
+Definition check_milp_def:
+  check_milp milp sol =
+  let solc = mk_sol sol in
+  EVERY (satisfies_milc solc) milp
+End
+
+Definition check_obj_def:
+  check_obj obj r sol =
+  let solc = mk_sol sol in
+  eval_lhs solc obj = r
+End
+
+Definition check_sol_def:
+  check_sol intv milp obj r (sol: real num_map) ⇔
+  check_dom intv sol ∧
+  check_milp milp sol ∧
+  check_obj obj r sol
+End
+
+(* Syntactic formulae are given by a sptree of (milc list, milc) *)
+Datatype:
+  vipr = Assum milc
+End
+
+(* Check that a given LHS is int valued *)
+Definition int_valued_def:
+  int_valued intv lhs ⇔
+  let xs = toAList lhs in
+  EVERY (λ(x,r). IS_SOME (lookup x intv) ∧ is_int r) xs
+End
+
+Definition round_milc_def:
+  round_milc intv (lop,lhs,n) =
+  if int_valued intv lhs then
+    case lop of
+      GreaterEqual => SOME (lop,lhs,real_of_int (INT_CEILING n))
+    | LessEqual => SOME (lop,lhs,real_of_int (INT_FLOOR n))
+    | _ => NONE
   else NONE
 End
 
-Theorem INT_FLOOR_real_of_int:
-  INT_FLOOR (real_of_int i) = i
+Definition absurdity_def:
+  absurdity ((lop,xs,n):milc) ⇔
+  xs = LN ∧
+  case lop of
+    GreaterEqual => n > 0
+  | LessEqual => n < 0
+  | Equal => n ≠ 0
+End
+
+Theorem absurdity_unsat:
+  absurdity milc ⇒
+  ¬satisfies_milc w milc
 Proof
+  PairCases_on`milc`>>
+  simp[absurdity_def,satisfies_milc_def,eval_lhs_def]>>
+  EVAL_TAC>>
+  every_case_tac>>fs[do_op_def,realaxTheory.real_ge]>>
+  PURE_REWRITE_TAC[realaxTheory.REAL_NOT_LE]>>
+  fs[realaxTheory.real_gt]
+QED
+
+(* c1 dominates c2 *)
+Definition dominates_def:
+  dominates (lop1,xs1,n1) (lop2,xs2,n2) ⇔
+  absurdity (lop1,xs1,n1) ∨
+  xs1 = xs2 ∧
+  case lop2 of
+    GreaterEqual =>
+    (lop1 = GreaterEqual ∨ lop1 = Equal) ∧ n1 ≥ n2
+  | LessEqual =>
+    (lop1 = LessEqual ∨ lop1 = Equal) ∧ n1 ≤ n2
+  | Equal =>
+    lop1 = Equal ∧ n1 = n2
+End
+
+Theorem dominates_imp:
+  dominates milc1 milc2 ∧
+  satisfies_milc w milc1 ⇒
+  satisfies_milc w milc2
+Proof
+  PairCases_on`milc1`>>
+  PairCases_on`milc2`>>
+  rw[dominates_def]
+  >-
+    metis_tac[absurdity_unsat]>>
+  every_case_tac>>fs[satisfies_milc_def]>>rw[]>>
+  fs[do_op_def]>>
+  metis_tac[realTheory.REAL_LE_TRANS,realaxTheory.real_ge]
+QED
+
+Definition check_vipr_def:
+  check_vipr fml id (Assum milc) =
+    SOME (insert id ([id],milc) fml, id+1)
+End
+
+Theorem is_int_add_mul:
+  is_int x ∧ is_int y ⇒
+  is_int (x + y) ∧
+  is_int (x * y)
+Proof
+  fs[intrealTheory.is_int_def]>>
+  rw[]>>
+  qpat_x_assum`_ = _` SUBST_ALL_TAC>>
+  qpat_x_assum`_ = _` SUBST_ALL_TAC>>
+  simp[intrealTheory.INT_FLOOR_SUM]>>
+  simp[INT_FLOOR_real_of_int]>>
+  simp[realTheory.REAL_ADD_COMM]>>
+  REWRITE_TAC[GSYM intrealTheory.real_of_int_mul]>>
   simp[intrealTheory.INT_FLOOR]
 QED
 
-Theorem rSUM_is_int:
-  ∀ys.
-  EVERY (λ(r,y). RAT_is_int r) ys ⇒
-  is_int (rSUM (MAP (eval_int_term w) ys))
+Theorem int_valued_is_int:
+  (∀v. v ∈ domain intv ⇒ is_int (w v)) ∧
+  int_valued intv milc
+  ⇒
+  is_int (eval_lhs w milc)
 Proof
-  Induct>>rw[rSUM_def]
+  rw[int_valued_def,eval_lhs_def]>>
+  rename1`is_int (rSUM (MAP _ ls))`>>
+  Induct_on`ls`>>fs[rSUM_def]
   >-
     EVAL_TAC>>
-  pairarg_tac>>fs[]>>
-  fs[intrealTheory.is_int_def,RAT_is_int_def]>>
+  rw[]>>fs[]>>
+  Cases_on`h`>>
+  fs[eval_real_term_def,domain_lookup,IS_SOME_EXISTS,PULL_EXISTS]>>
+  first_x_assum drule>>
   rw[]>>
-  simp[eval_int_term_def]>>
-  qpat_x_assum`_ = _` SUBST_ALL_TAC>>
-  qpat_x_assum`_ = _` SUBST_ALL_TAC>>
-  simp[intrealTheory.INT_FLOOR_SUM, GSYM real_of_int_of_rat]>>
-  REWRITE_TAC[GSYM intrealTheory.real_of_int_mul]>>
-  simp[INT_FLOOR_real_of_int]
+  metis_tac[is_int_add_mul]
 QED
 
 Theorem le_real_of_int:
@@ -158,27 +261,161 @@ Proof
   intLib.ARITH_TAC
 QED
 
-Theorem round_up_sound:
-  satisfies_milc w (GreaterEqual,cs,rhs) ∧
-  round_up (cs,rhs) = SOME rhs' ⇒
-  satisfies_milc w (GreaterEqual,cs,rhs')
+Theorem round_up:
+  is_int r ∧
+  r ≥ f ⇒ r ≥ real_of_int (INT_CEILING f)
 Proof
-  rw[satisfies_milc_def]>>
-  Cases_on`cs`>>
-  fs[round_up_def]>>rw[]>>
-  Cases_on`w`>>fs[eval_lhs_def,rSUM_def,realTheory.real_ge]>>
-  rename1`eval_int_term w`>>
-  drule rSUM_is_int >>
-  disch_then(qspec_then`w` assume_tac)>>
-  simp[GSYM real_of_int_of_rat]>>
-  rename1`is_int ri`>>
-  fs[RAT_INT_CEILING_def]>>
+  rw[]>>
   fs[intrealTheory.is_int_def]>>
-  pop_assum SUBST_ALL_TAC>>
-  gs[]>>
-  metis_tac[le_real_of_int]
+  fs[realaxTheory.real_ge]>>
+  `INT_CEILING f ≤ INT_FLOOR r` by metis_tac[le_real_of_int]>>
+  `real_of_int (INT_FLOOR r) ≤ r` by
+    metis_tac[intrealTheory.INT_FLOOR_BOUNDS]>>
+  metis_tac[intrealTheory.real_of_int_le,realaxTheory.REAL_LE_TRANS]
 QED
 
-(* TODO: addition runs into annoying canonicalization again *)
+Theorem real_of_int_le:
+  real_of_int i ≤ r ⇒
+  i ≤ INT_FLOOR r
+Proof
+  rw[]>>
+  CCONTR_TAC>>
+  fs[integerTheory.INT_NOT_LE]>>
+  `r < real_of_int (INT_FLOOR r + 1)` by
+    metis_tac[intrealTheory.INT_FLOOR]>>
+  `real_of_int i < real_of_int (INT_FLOOR r + 1)` by
+    metis_tac[realaxTheory.REAL_LET_TRANS]>>
+  fs[]>>
+  intLib.ARITH_TAC
+QED
+
+Theorem round_down:
+  is_int r ∧
+  r ≤ f ⇒ r ≤ real_of_int (INT_FLOOR f)
+Proof
+  rw[]>>
+  fs[intrealTheory.is_int_def]>>
+  `INT_FLOOR r ≤ INT_FLOOR f` by metis_tac[real_of_int_le]>>
+  metis_tac[intrealTheory.real_of_int_le,realaxTheory.REAL_LE_TRANS]
+QED
+
+Theorem round_milc_sound:
+  (∀v. v ∈ domain intv ⇒ is_int (w v)) ∧
+  satisfies_milc w milc ∧
+  round_milc intv milc = SOME milc'
+  ⇒
+  satisfies_milc w milc'
+Proof
+  PairCases_on`milc`>>fs[round_milc_def]>>
+  TOP_CASE_TAC>>rw[]>>
+  fs[satisfies_milc_def]
+  >- (
+    match_mp_tac round_up>>
+    fs[]>>
+    metis_tac[int_valued_is_int])>>
+  match_mp_tac round_down>>
+  fs[]>>
+  metis_tac[int_valued_is_int]
+QED
+
+(* Lookup the assumptions corresponding to the list of indices *)
+Definition get_assms_def:
+  get_assms (fml: (num list # milc) num_map) (ls,c) =
+  (set (MAP (λid. SND (THE (lookup id fml))) ls),c)
+End
+
+Definition range_def:
+  range s = {v | ∃n. lookup n s = SOME v}
+End
+
+Theorem range_delete:
+  range (delete h v) ⊆ range v
+Proof
+  simp[range_def,lookup_delete,SUBSET_DEF]>>
+  metis_tac[]
+QED
+
+Theorem range_insert:
+  n ∉ domain fml ⇒
+  range (insert n l fml) = l INSERT range fml
+Proof
+  rw[range_def,EXTENSION,lookup_insert,domain_lookup]>>
+  metis_tac[SOME_11]
+QED
+
+Theorem range_insert_2:
+  C ∈ range (insert n l fml) ⇒ C ∈ range fml ∨ C = l
+Proof
+  fs[range_def,lookup_insert]>>
+  rw[]>>
+  every_case_tac>>fs[]>>
+  metis_tac[]
+QED
+
+Theorem range_insert_SUBSET:
+  range (insert n l fml) ⊆ l INSERT range fml
+Proof
+  rw[SUBSET_DEF]>>
+  metis_tac[range_insert_2]
+QED
+
+(* The only allowed assumptions must be "self-loops" *)
+Definition is_assm_def:
+  is_assm fml id ⇔
+  case lookup id fml of
+    NONE => F
+  | SOME (assms,c) => assms = [id]
+End
+
+Definition good_fml_def:
+  good_fml fml ⇔
+  ∀asmc.
+    asmc ∈ range fml ⇒
+    EVERY (is_assm fml) (FST asmc)
+End
+
+Definition id_ok_def:
+  id_ok fml id ⇔
+  ∀n. id ≤ n ⇒ n ∉ domain fml
+End
+
+(* check the main body of a VIPR proof *)
+Theorem check_vipr_sound:
+  check_vipr fml id vipr = SOME (fml',id') ∧
+  id_ok fml id ∧
+  good_fml fml ∧
+  satisfies_imp_milp w (IMAGE (get_assms fml) (range fml)) ⇒
+  satisfies_imp_milp w (IMAGE (get_assms fml') (range fml'))
+Proof
+  Cases_on`vipr`>>rw[check_vipr_def]
+  >- (
+    fs[satisfies_imp_milp_def]>>
+    rw[]>>
+    Cases_on`x`>>fs[get_assms_def]>>rw[]>>
+    pop_assum mp_tac>>
+    DEP_REWRITE_TAC [range_insert]>>
+    fs[id_ok_def]>>
+    rw[]
+    >-
+      (fs[]>>rw[satisfies_imp_milc_def])>>
+    fs[good_fml_def]>>
+    first_x_assum drule>>rw[]>>
+    fs[PULL_EXISTS]>>
+    first_x_assum (drule_at Any)>>
+    simp[get_assms_def]>>rw[]>>
+    fs[satisfies_imp_milc_def,MEM_MAP,lookup_insert,PULL_EXISTS]>>
+    rw[]>>
+    first_x_assum match_mp_tac>>
+    rw[]>>
+    first_x_assum drule>>
+    fs[EVERY_MEM]>>
+    `id' ≠ id` by (
+      first_x_assum drule>>
+      fs[is_assm_def,domain_lookup]>>
+      every_case_tac>>rw[]>>
+      first_x_assum(qspec_then`id` assume_tac)>>fs[]>>
+      metis_tac[option_CLAUSES])>>
+    simp[])
+QED
 
 val _ = export_theory();
